Interface changes to HaCl

crypto_hst/HaCl.fst
@@ -1,7 +1,13 @@
 module HaCl
 
-open FStar.HyperStack
 open HaCl.Base
+
+//open Hash.Sha1
+//open Hash.Sha224
+open Hash.Sha256
+//open Hash.Sha384
+//open Hash.Sha512
+
 
 
 ////////////////////////////////////////////////////////////////// 
@@ -11,10 +17,14 @@ open HaCl.Base
 
 assume val hacl_hash': alg:hash_alg -> data:bytes -> len:bytes{len = length data} -> Tot (hash:bytes{length hash = hashSize alg})
 
-val hacl_hash: alg:hash_alg -> hash:bytes{length hash = hashSize alg} -> data:bytes -> len:nat{len = length data} 
-  -> STL (retcode:int)
-        (requires (fun h -> live h hash /\ live h data))
-        (ensures  (fun h0 r h1 -> live h1 hash /\ live h1 data /\ modifies_1 hash h0 h1 /\ hash = (hacl_hash' alg data len)))
+let hacl_hash alg hash data len =
+  match alg with
+//  | SHA1 -> sha1 hash data len
+//  | SHA224 -> sha224 hash data len
+  | SHA256 -> sha256 hash data len 
+//  | SHA384 -> sha384 hash data len 
+//  | SHA512 -> sha512 hash data len
+
 
 
 ////////////////////////////////////////////////////////////////// 
@@ -28,23 +38,12 @@ val hacl_hash: alg:hash_alg -> hash:bytes{length hash = hashSize alg} -> data:by
 
 assume val hacl_secretbox': alg:aead_alg -> input:bytes -> len:nat{len = length input} -> n:nonce{length n = aeadRealIVSize alg} -> k:key{length k = aeadKeySize alg} -> Tot (output:ciphertext{length output = len})
 
-val hacl_secretbox: alg:aead_alg -> output:ciphertext -> input:bytes -> len:nat{len = length input} -> n:nonce{length n = aeadRealIVSize alg} -> k:key{length k = aeadKeySize alg}
-  -> STL (retcode:int)
-        (requires (fun h -> live h output /\ live h input /\ live h n /\ live h k))
-        (ensures  (fun h0 r h1 -> live h1 output /\ live h1 input /\ live h1 n /\ live h1 k 
-                             /\ modifies_1 output h0 h1 /\ output = (hacl_secretbox' alg input len n k)))
 
 //
 // Function : crypto_secretbox_open
 //
 
 assume val hacl_secretbox_open': alg:aead_alg -> input:ciphertext -> len:nat{len = length input} -> n:nonce{length n = aeadRealIVSize alg} -> k:key{length k = aeadKeySize alg} -> Tot (output:bytes{length output = len})
-
-val hacl_secretbox_open: alg:aead_alg -> output:bytes -> input:ciphertext -> len:nat{len = length input} -> n:nonce{length n = aeadRealIVSize alg} -> k:key{length k = aeadKeySize alg} 
-  -> STL (retcode:int)
-        (requires (fun h -> live h output /\ live h input /\ live h n /\ live h k))
-        (ensures  (fun h0 r h1 -> live h1 output /\ live h1 input /\ live h1 n /\ live h1 k
-                             /\ modifies_1 output h0 h1 /\ output = (hacl_secretbox_open' alg input len n k)))
 
 
 ////////////////////////////////////////////////////////////////// 
@@ -58,13 +57,6 @@ val hacl_secretbox_open: alg:aead_alg -> output:bytes -> input:ciphertext -> len
 
 assume val hacl_box_keypair': ec:ec_curve -> Tot (pk:ec_point{ec_point_is_on_curve ec pkey} * sk:ec_key{ec_point_is_pkey_of_skey ec skey pkey})
 
-val hacl_box_keypair: ec:ec_curve -> pkey:ec_point_bytes -> skey:ec_key_bytes 
-  -> STL (retcode:int)
-        (requires (fun h -> live h pkey /\ live h skey))
-        (ensures  (fun h0 r h1 -> live h1 pkey /\ live h1 skey 
-                             /\ modifies_1 pkey h0 h1 /\ modifies_2 skey h0 h1
-                             /\ pkey = serialize_ec_point (first (hacl_box_keypair' ()))
-                             /\ skey = serialize_ec_key (snd (hacl_box_keypair' ()))))
 
 //
 // Function : crypto_box
@@ -72,22 +64,9 @@ val hacl_box_keypair: ec:ec_curve -> pkey:ec_point_bytes -> skey:ec_key_bytes
 
 assume val hacl_box': ec:ec_curve -> alg:aead_cipher -> input:bytes -> len:nat{len = length input} -> n:nonce{length n = aeadRealIVSize alg} -> pkey:ec_point{ec_point_is_on_curve ec pkey} -> skey:ec_key{ec_point_is_pkey_of_skey ec skey pkey} -> Tot (output:ciphertext{length output = len})
 
-val hacl_box: ec:ec_curve -> alg:aead_cipher -> output:ciphertext -> input:bytes -> len:nat{len = length input} -> n:nonce{length n = aeadRealIVSize alg} -> pkey:ec_point_bytes -> skey:ec_key_bytes
-  -> STL (retcode:int)
-        (requires (fun h -> live h output /\ live h input /\ live h n /\ live h pkey /\ live h skey))
-        (ensures  (fun h0 r h1 -> live h1 output /\ live h1 input /\ live h1 n /\ live h1 pkey /\ live h1 skey
-                             /\ modifies_1 output h0 h1 
-                             /\ output = (hacl_box' ec alg input len n (parsing_ec_point pkey) (parsing_ec_key skey))))
 
 //
 // Function : crypto_box_open
 //
 
 assume val hacl_box_open': ec:ec_curve -> alg:aead_alg -> input:ciphertext -> len:nat{len = length ciphertext} -> n:nonce{length n = aeadRealIVSize alg} -> pkey:ec_point{ec_point_is_on_curve ec pkey} -> skey:ec_key{ec_point_is_pkey_of_skey ec skey pkey} -> Tot (output:bytes{length output = len})
-
-val hacl_box_open: ec:ec_curve -> alg:aead_cipher -> output:bytes -> input:ciphertext -> len:nat{len = length ciphertext} -> n:nonce{length n = aeadRealIVSize alg} -> pkey:ec_point_bytes -> skey:ec_key_bytes
-  -> STL (retcode:int)
-        (requires (fun h -> live h output /\ live h input /\ live h n /\ live h pkey /\ live h skey))
-        (ensures  (fun h0 r h1 -> live h1 output /\ live h1 input /\ live h1 n /\ live h1 pkey /\ live h1 skey
-                             /\ modifies_1 output h0 h1
-                             /\ output = (hacl_box_open' ec alg input len n (parsing_ec_point pkey) (parsing_ec_key skey))))
