crypto_hst/HaCl.fsti
@@ -1,0 +1,81 @@
+module HaCl
+
+open FStar.HyperStack
+open HaCl.Base
+
+
+////////////////////////////////////////////////////////////////// 
+//
+// Hashing functions
+//
+
+val hacl_hash: alg:hash_alg -> hash:bytes{length hash = hashSize alg} -> data:bytes -> len:nat{len = length data} 
+  -> STL (retcode:int)
+        (requires (fun h -> live h hash /\ live h data))
+        (ensures  (fun h0 r h1 -> live h1 hash /\ live h1 data /\ modifies_1 hash h0 h1 /\ hash = (hacl_hash' alg data len)))
+
+
+////////////////////////////////////////////////////////////////// 
+//
+// Authenticated encryption functions for secret-key cryptography
+//
+
+//
+// Function : crypto_secretbox
+//
+
+assume val hacl_secretbox: alg:aead_alg -> output:ciphertext -> input:bytes -> len:nat{len = length input} -> n:nonce{length n = aeadRealIVSize alg} -> k:key{length k = aeadKeySize alg}
+  -> STL (retcode:int)
+        (requires (fun h -> live h output /\ live h input /\ live h n /\ live h k))
+        (ensures  (fun h0 r h1 -> live h1 output /\ live h1 input /\ live h1 n /\ live h1 k 
+                             /\ modifies_1 output h0 h1 /\ output = (hacl_secretbox' alg input len n k)))
+
+//
+// Function : crypto_secretbox_open
+//
+
+assume val hacl_secretbox_open: alg:aead_alg -> output:bytes -> input:ciphertext -> len:nat{len = length input} -> n:nonce{length n = aeadRealIVSize alg} -> k:key{length k = aeadKeySize alg} 
+  -> STL (retcode:int)
+        (requires (fun h -> live h output /\ live h input /\ live h n /\ live h k))
+        (ensures  (fun h0 r h1 -> live h1 output /\ live h1 input /\ live h1 n /\ live h1 k
+                             /\ modifies_1 output h0 h1 /\ output = (hacl_secretbox_open' alg input len n k)))
+
+
+////////////////////////////////////////////////////////////////// 
+//
+// Authenticated encryption functions for public-key cryptography
+//
+
+//
+// Function : crypto_box_keypair
+//
+
+assume val hacl_box_keypair: ec:ec_curve -> pkey:ec_point_bytes -> skey:ec_key_bytes 
+  -> STL (retcode:int)
+        (requires (fun h -> live h pkey /\ live h skey))
+        (ensures  (fun h0 r h1 -> live h1 pkey /\ live h1 skey 
+                             /\ modifies_1 pkey h0 h1 /\ modifies_2 skey h0 h1
+                             /\ pkey = serialize_ec_point (first (hacl_box_keypair' ()))
+                             /\ skey = serialize_ec_key (snd (hacl_box_keypair' ()))))
+
+//
+// Function : crypto_box
+//
+
+assume val hacl_box: ec:ec_curve -> alg:aead_cipher -> output:ciphertext -> input:bytes -> len:nat{len = length input} -> n:nonce{length n = aeadRealIVSize alg} -> pkey:ec_point_bytes -> skey:ec_key_bytes
+  -> STL (retcode:int)
+        (requires (fun h -> live h output /\ live h input /\ live h n /\ live h pkey /\ live h skey))
+        (ensures  (fun h0 r h1 -> live h1 output /\ live h1 input /\ live h1 n /\ live h1 pkey /\ live h1 skey
+                             /\ modifies_1 output h0 h1 
+                             /\ output = (hacl_box' ec alg input len n (parsing_ec_point pkey) (parsing_ec_key skey))))
+
+//
+// Function : crypto_box_open
+//
+
+assume val hacl_box_open: ec:ec_curve -> alg:aead_cipher -> output:bytes -> input:ciphertext -> len:nat{len = length ciphertext} -> n:nonce{length n = aeadRealIVSize alg} -> pkey:ec_point_bytes -> skey:ec_key_bytes
+  -> STL (retcode:int)
+        (requires (fun h -> live h output /\ live h input /\ live h n /\ live h pkey /\ live h skey))
+        (ensures  (fun h0 r h1 -> live h1 output /\ live h1 input /\ live h1 n /\ live h1 pkey /\ live h1 skey
+                             /\ modifies_1 output h0 h1
+                             /\ output = (hacl_box_open' ec alg input len n (parsing_ec_point pkey) (parsing_ec_key skey))))
